Arithmetization/ISigmaOne/Metamath/Formula/Functions.lean
@@ -61,6 +61,26 @@ def Language.neg (p : V) : V := (construction L).result 0 p
 
 variable {L}
 
+section
+
+def _root_.LO.FirstOrder.Arith.LDef.negDef (pL : LDef) : 𝚺₁-Semisentence 2 := (blueprint pL).result.rew (Rew.substs ![#0, ‘0’, #1])
+
+variable (L)
+
+lemma neg_defined : 𝚺₁-Function₁ L.neg via pL.negDef := fun v ↦ by
+  simpa [LDef.negDef] using (construction L).result_defined ![v 0, 0, v 1]
+
+@[simp] lemma neg_defined_iff (v : Fin 2 → V) :
+    Semiformula.Evalbm (L := ℒₒᵣ) V v pL.negDef ↔ v 0 = L.neg (v 1) := (neg_defined L).df.iff v
+
+instance neg_definable : 𝚺₁-Function₁ L.neg :=
+  Defined.to_definable _ (neg_defined L)
+
+@[simp, definability] instance neg_definable' (Γ) : (Γ, m + 1)-Function₁ L.neg :=
+  .of_sigmaOne (neg_definable L) _ _
+
+end
+
 @[simp] lemma neg_rel {n k R v} (hR : L.Rel k R) (hv : L.SemitermSeq k n v) :
     L.neg (^rel n k R v) = ^nrel n k R v := by simp [Language.neg, hR, hv, construction]
 
@@ -84,26 +104,6 @@ variable {L}
 
 @[simp] lemma neg_ex {n p} (hp : L.Semiformula (n + 1) p) :
     L.neg (^∃[n] p) = ^∀[n] (L.neg p) := by simp [Language.neg, hp, construction]
-
-section
-
-def _root_.LO.FirstOrder.Arith.LDef.negDef (pL : LDef) : 𝚺₁-Semisentence 2 := (blueprint pL).result.rew (Rew.substs ![#0, ‘0’, #1])
-
-variable (L)
-
-lemma neg_defined : 𝚺₁-Function₁ L.neg via pL.negDef := fun v ↦ by
-  simpa [LDef.negDef] using (construction L).result_defined ![v 0, 0, v 1]
-
-@[simp] lemma neg_defined_iff (v : Fin 2 → V) :
-    Semiformula.Evalbm (L := ℒₒᵣ) V v pL.negDef ↔ v 0 = L.neg (v 1) := (neg_defined L).df.iff v
-
-instance neg_definable : 𝚺₁-Function₁ L.neg :=
-  Defined.to_definable _ (neg_defined L)
-
-@[simp, definability] instance neg_definable' (Γ) : (Γ, m + 1)-Function₁ L.neg :=
-  .of_sigmaOne (neg_definable L) _ _
-
-end
 
 @[simp] lemma Language.Semiformula.neg {p : V} : L.Semiformula n p → L.Semiformula n (L.neg p) := by
   apply Language.Semiformula.induction_sigma₁
@@ -167,46 +167,158 @@ end
 namespace Substs
 
 def blueprint (pL : LDef) : Language.UformulaRec1.Blueprint pL where
-  rel    := .mkSigma “y param n k R v m w | ∃ v', !pL.termSubstSeqDef k n m w v v' ∧ !qqRelDef y m k R v'” (by simp)
-  nrel   := .mkSigma “y param n k R v m w | ∃ v', !pL.termSubstSeqDef k n m w v v' ∧ !qqNRelDef y m k R v'” (by simp)
-  verum  := .mkSigma “y param n m w | !qqVerumDef y m” (by simp)
-  falsum := .mkSigma “y param n m w | !qqFalsumDef y m” (by simp)
-  and    := .mkSigma “y param n p₁ p₂ y₁ y₂ m w | !qqAndDef y m y₁ y₂” (by simp)
-  or     := .mkSigma “y param n p₁ p₂ y₁ y₂ m w | !qqOrDef y m y₁ y₂” (by simp)
-  all    := .mkSigma “y param n p₁ y₁ m w | !qqAllDef y m y₁” (by simp)
-  ex     := .mkSigma “y param n p₁ y₁ m w | !qqExDef y m y₁” (by simp)
-  allChanges := .mkSigma “w' w n | ” (by simp)
+  rel    := .mkSigma “y param n k R v | ∃ m, !pi₁Def m param ∧ ∃ w, !pi₂Def w param ∧ ∃ v', !pL.termSubstSeqDef v' k n m w v ∧ !qqRelDef y m k R v'” (by simp)
+  nrel   := .mkSigma “y param n k R v | ∃ m, !pi₁Def m param ∧ ∃ w, !pi₂Def w param ∧ ∃ v', !pL.termSubstSeqDef v' k n m w v ∧ !qqNRelDef y m k R v'” (by simp)
+  verum  := .mkSigma “y param n | ∃ m, !pi₁Def m param ∧ !qqVerumDef y m” (by simp)
+  falsum := .mkSigma “y param n | ∃ m, !pi₁Def m param ∧ !qqFalsumDef y m” (by simp)
+  and    := .mkSigma “y param n p₁ p₂ y₁ y₂ | ∃ m, !pi₁Def m param ∧ !qqAndDef y m y₁ y₂” (by simp)
+  or     := .mkSigma “y param n p₁ p₂ y₁ y₂ | ∃ m, !pi₁Def m param ∧ !qqOrDef y m y₁ y₂” (by simp)
+  all    := .mkSigma “y param n p₁ y₁ | ∃ m, !pi₁Def m param ∧ !qqAllDef y m y₁” (by simp)
+  ex     := .mkSigma “y param n p₁ y₁ | ∃ m, !pi₁Def m param ∧ !qqExDef y m y₁” (by simp)
+  allChanges := .mkSigma “param' param n | ∃ m, !pi₁Def m param ∧ ∃ w, !pi₂Def w param ∧ ∃ qseq, !pL.qSeqDef qseq n m w ∧ !pairDef param' (m + 1) qseq” (by simp)
+  exChanges := .mkSigma “param' param n | ∃ m, !pi₁Def m param ∧ ∃ w, !pi₂Def w param ∧ ∃ qseq, !pL.qSeqDef qseq n m w ∧ !pairDef param' (m + 1) qseq” (by simp)
 
-/--/
 variable (L)
 
-def construction : Language.UformulaRec.Construction V L (blueprint pL) where
-  rel    {param} := fun n k R v ↦ ^rel (param 0) k R (L.termSubstSeq k n (param 0) (param 1) v)
-  nrel   {param} := fun n k R v ↦ ^nrel (param 0) k R (L.termSubstSeq k n (param 0) (param 1) v)
-  verum  {param} := fun n ↦ ^⊤[param 0]
-  falsum {param} := fun n ↦ ^⊥[param 0]
-  and    {param} := fun n _ _ y₁ y₂ ↦ y₁ ^⋎[param 0] y₂
-  or     {param} := fun n _ _ y₁ y₂ ↦ y₁ ^⋏[param 0] y₂
-  all    {param} := fun n _ y₁ ↦ ^∀[param 0] y₁
-  ex     {param} := fun n _ y₁ ↦ ^∃[param 0] y₁
-
-  nrel {_} := fun n k R v ↦ ^rel n k R v
-  verum {_} := fun n ↦ ^⊥[n]
-  falsum {_} := fun n ↦ ^⊤[n]
-  and {_} := fun n _ _ y₁ y₂ ↦ y₁ ^⋎[n] y₂
-  or {_} := fun n _ _ y₁ y₂ ↦ y₁ ^⋏[n] y₂
-  all {_} := fun n _ y₁ ↦ ^∃[n] y₁
-  ex {_} := fun n _ y₁ ↦ ^∀[n] y₁
-  rel_defined := by intro v; simp [blueprint]; rfl
-  nrel_defined := by intro v; simp [blueprint]; rfl
+def construction : Language.UformulaRec1.Construction V L (blueprint pL) where
+  rel (param) := fun n k R v ↦ ^rel (π₁ param) k R (L.termSubstSeq k n (π₁ param) (π₂ param) v)
+  nrel (param) := fun n k R v ↦ ^nrel (π₁ param) k R (L.termSubstSeq k n (π₁ param) (π₂ param) v)
+  verum (param) := fun _ ↦ ^⊤[π₁ param]
+  falsum (param) := fun _ ↦ ^⊥[π₁ param]
+  and (param) := fun _ _ _ y₁ y₂ ↦ y₁ ^⋏[π₁ param] y₂
+  or (param) := fun _ _ _ y₁ y₂ ↦ y₁ ^⋎[π₁ param] y₂
+  all (param) := fun _ _ y₁ ↦ ^∀[π₁ param] y₁
+  ex (param) := fun _ _ y₁ ↦ ^∃[π₁ param] y₁
+  allChanges (param n) := ⟪π₁ param + 1, L.qSeq n (π₁ param) (π₂ param)⟫
+  exChanges (param n) := ⟪π₁ param + 1, L.qSeq n (π₁ param) (π₂ param)⟫
+  rel_defined := by intro v; simp [blueprint, (termSubstSeq_defined L).df.iff]; rfl
+  nrel_defined := by intro v; simp [blueprint, (termSubstSeq_defined L).df.iff]; rfl
   verum_defined := by intro v; simp [blueprint]
   falsum_defined := by intro v; simp [blueprint]
   and_defined := by intro v; simp [blueprint]; rfl
   or_defined := by intro v; simp [blueprint]; rfl
-  all_defined := by intro v
--/
+  all_defined := by intro v; simp [blueprint]; rfl
+  ex_defined := by intro v; simp [blueprint]; rfl
+  allChanges_defined := by intro v; simp [blueprint, (qSeq_defined L).df.iff]
+  exChanges_defined := by intro v; simp [blueprint, (qSeq_defined L).df.iff]
 
+end Substs
 
+open Substs
+
+variable (L)
+
+def Language.substs (m w p : V) : V := (construction L).result ⟪m, w⟫ p
+
+variable {L}
+
+section
+
+def _root_.LO.FirstOrder.Arith.LDef.substsDef (pL : LDef) : 𝚺₁-Semisentence 4 := .mkSigma
+  “q m w p | ∃ mw, !pairDef mw m w ∧ !(blueprint pL).result q mw p” (by simp)
+
+variable (L)
+
+lemma substs_defined : 𝚺₁-Function₃ L.substs via pL.substsDef := fun v ↦ by
+  simp [LDef.substsDef, (construction L).result_defined.df.iff]; rfl
+
+@[simp] lemma eval_substsDef (v : Fin 4 → V) :
+    Semiformula.Evalbm (L := ℒₒᵣ) V v pL.substsDef ↔ v 0 = L.substs (v 1) (v 2) (v 3) := (substs_defined L).df.iff v
+
+instance substs_definable : 𝚺₁-Function₃ L.substs :=
+  Defined.to_definable _ (substs_defined L)
+
+@[simp, definability] instance substs_definable' (Γ) : (Γ, m + 1)-Function₃ L.substs :=
+  .of_sigmaOne (substs_definable L) _ _
+
+end
+
+variable {m w : V}
+
+@[simp] lemma substs_rel {n k R v} (hR : L.Rel k R) (hv : L.SemitermSeq k n v) :
+    L.substs m w (^rel n k R v) = ^rel m k R (L.termSubstSeq k n m w v) := by simp [Language.substs, hR, hv, construction]
+
+@[simp] lemma substs_nrel {n k R v} (hR : L.Rel k R) (hv : L.SemitermSeq k n v) :
+    L.substs m w (^nrel n k R v) = ^nrel m k R (L.termSubstSeq k n m w v) := by simp [Language.substs, hR, hv, construction]
+
+@[simp] lemma substs_verum (n) :
+    L.substs m w ^⊤[n] = ^⊤[m] := by simp [Language.substs, construction]
+
+@[simp] lemma substs_falsum (n) :
+    L.substs m w ^⊥[n] = ^⊥[m] := by simp [Language.substs, construction]
+
+@[simp] lemma substs_and {n p q} (hp : L.Semiformula n p) (hq : L.Semiformula n q) :
+    L.substs m w (p ^⋏[n] q) = L.substs m w p ^⋏[m] L.substs m w q := by simp [Language.substs, hp, hq, construction]
+
+@[simp] lemma substs_or {n p q} (hp : L.Semiformula n p) (hq : L.Semiformula n q) :
+    L.substs m w (p ^⋎[n] q) = L.substs m w p ^⋎[m] L.substs m w q := by simp [Language.substs, hp, hq, construction]
+
+@[simp] lemma substs_all {n p} (hp : L.Semiformula (n + 1) p) :
+    L.substs m w (^∀[n] p) = ^∀[m] (L.substs (m + 1) (L.qSeq n m w) p) := by simp [Language.substs, hp, construction]
+
+@[simp] lemma substs_ex {n p} (hp : L.Semiformula (n + 1) p) :
+    L.substs m w (^∃[n] p) = ^∃[m] (L.substs (m + 1) (L.qSeq n m w) p) := by simp [Language.substs, hp, construction]
+
+lemma semiformula_subst_induction {P : V → V → V → V → V → Prop} (hP : 𝚺₁-Relation₅ P)
+    (hRel : ∀ n m w k R v, L.Rel k R → L.SemitermSeq k n v → P n m w (^rel n k R v) (^rel m k R (L.termSubstSeq k n m w v)))
+    (hNRel : ∀ n m w k R v, L.Rel k R → L.SemitermSeq k n v → P n m w (^nrel n k R v) (^nrel m k R (L.termSubstSeq k n m w v)))
+    (hverum : ∀ n m w, P n m w (^⊤[n]) (^⊤[m]))
+    (hfalsum : ∀ n m w, P n m w (^⊥[n]) (^⊥[m]))
+    (hand : ∀ n m w p q, L.Semiformula n p → L.Semiformula n q →
+      P n m w p (L.substs m w p) → P n m w q (L.substs m w q) → P n m w (p ^⋏[n] q) (L.substs m w p ^⋏[m] L.substs m w q))
+    (hor : ∀ n m w p q, L.Semiformula n p → L.Semiformula n q →
+      P n m w p (L.substs m w p) → P n m w q (L.substs m w q) → P n m w (p ^⋎[n] q) (L.substs m w p ^⋎[m] L.substs m w q))
+    (hall : ∀ n m w p, L.Semiformula (n + 1) p →
+      P (n + 1) (m + 1) (L.qSeq n m w) p (L.substs (m + 1) (L.qSeq n m w) p) →
+      P n m w (^∀[n] p) (^∀[m] (L.substs (m + 1) (L.qSeq n m w) p)))
+    (hex : ∀ n m w p, L.Semiformula (n + 1) p →
+      P (n + 1) (m + 1) (L.qSeq n m w) p (L.substs (m + 1) (L.qSeq n m w) p) →
+      P n m w (^∃[n] p) (^∃[m] (L.substs (m + 1) (L.qSeq n m w) p))) :
+    ∀ {n p m w}, L.Semiformula n p → P n m w p (L.substs m w p) := by
+  suffices ∀ param n p, L.Semiformula n p → P n (π₁ param) (π₂ param) p ((construction L).result param p) by
+    intro n p m w hp; simpa using this ⟪m, w⟫ n p hp
+  apply (construction L).semiformula_result_induction (P := fun param n p y ↦ P n (π₁ param) (π₂ param) p y)
+  · apply Definable.comp₅'
+      (DefinableFunction.var _)
+      (DefinableFunction.comp₁ (DefinableFunction.var _))
+      (DefinableFunction.comp₁ (DefinableFunction.var _))
+      (DefinableFunction.var _)
+      (DefinableFunction.var _)
+  · intro param n k R v hkR hv; simpa using hRel n (π₁ param) (π₂ param) k R v hkR hv
+  · intro param n k R v hkR hv; simpa using hNRel n (π₁ param) (π₂ param) k R v hkR hv
+  · intro param n; simpa using hverum n (π₁ param) (π₂ param)
+  · intro param n; simpa using hfalsum n (π₁ param) (π₂ param)
+  · intro param n p q hp hq ihp ihq
+    simpa [Language.substs] using
+      hand n (π₁ param) (π₂ param) p q hp hq (by simpa [Language.substs] using ihp) (by simpa [Language.substs] using ihq)
+  · intro param n p q hp hq ihp ihq
+    simpa [Language.substs] using
+      hor n (π₁ param) (π₂ param) p q hp hq (by simpa [Language.substs] using ihp) (by simpa [Language.substs] using ihq)
+  · intro param n p hp ihp
+    simpa using hall n (π₁ param) (π₂ param) p hp (by simpa [construction] using ihp)
+  · intro param n p hp ihp
+    simpa using hex n (π₁ param) (π₂ param) p hp (by simpa [construction] using ihp)
+
+@[simp] lemma Language.Semiformula.substs {n p m w : V} :
+    L.Semiformula n p → L.SemitermSeq n m w → L.Semiformula m (L.substs m w p) := by
+  apply semiformula_subst_induction (P := fun n m w _ y ↦ L.SemitermSeq n m w → L.Semiformula m y)
+  · definability
+  case hRel => intro n m w k R v hR hv hw; simp [hR, hv, hw]
+  case hNRel => intro n m w k R v hR hv hw; simp [hR, hv, hw]
+  case hverum => simp
+  case hfalsum => simp
+  case hand =>
+    intro n m w p q _ _ ihp ihq hw
+    simp [ihp hw, ihq hw]
+  case hor =>
+    intro n m w p q _ _ ihp ihq hw
+    simp [ihp hw, ihq hw]
+  case hall =>
+    intro n m w p _ ih hw
+    simpa using ih hw.qSeq
+  case hex =>
+    intro n m w p _ ih hw
+    simpa using ih hw.qSeq
 
 end substs
 
